rename acyclic into idempotent

theories/mgu.v
@@ -4,11 +4,11 @@ From det Require Import finmap ctx.
 From det Require Import lang unif.
 
 Definition is_mgu (mgu s : Sigma) :=
-  exists2 r : Sigma, acyclic r &
+  exists2 r : Sigma, idempotent r &
       forall t, deref r (deref mgu t) = deref s t.
 
 Definition mgu_help base mgu l :=
-  forall s, acyclic s -> unifier s l -> is_mgu base s -> is_mgu mgu s.
+  forall s, idempotent s -> unifier s l -> is_mgu base s -> is_mgu mgu s.
 
 Lemma mgu_help_refl b l: mgu_help b b l.
 Proof. by move=> *. Qed.
@@ -58,7 +58,7 @@ Lemma buildr_in s t x (xs: x \in domf s) (xI: x \in domf s `&` vars t):
   (build_r s t) [`xI] = s.[xs].
 Proof. apply: buildrV_in. Qed.
 
-Lemma in_vars x r t: acyclic r -> x \in domf r -> x \in vars (deref r t) = false.
+Lemma in_vars x r t: idempotent r -> x \in domf r -> x \in vars (deref r t) = false.
 Proof.
   move=> A xr.
   elim: t => //=[v|f Hf a Ha]; last by rewrite inE Hf//.
@@ -67,7 +67,7 @@ Proof.
   by apply/codom_varsP; exists v, vr.
 Qed.
 
-Lemma in_vars_V x r v (vx : v \in domf r): acyclic r -> x \in domf r -> x \in vars r.[vx] = false.
+Lemma in_vars_V x r v (vx : v \in domf r): idempotent r -> x \in domf r -> x \in vars r.[vx] = false.
 Proof.
   move=> A xr; replace r.[vx] with (deref r (Tm_V v)) by rewrite/=in_fnd//.
   by rewrite in_vars.
@@ -105,7 +105,7 @@ Proof.
 Qed.
 
 Lemma is_mgu_deref_sigma v t mgu s (vs: v \in domf s):
-  acyclic mgu -> acyclic s -> v \notin vars t -> domf mgu # vars t ->
+  idempotent mgu -> idempotent s -> v \notin vars t -> domf mgu # vars t ->
   s.[vs] = deref s t -> v \notin domf mgu ->
   is_mgu mgu s -> is_mgu (deref_sigma v t mgu) s.
 Proof.
@@ -200,7 +200,7 @@ Proof.
 Qed.
 
 Lemma mgu_help_deref_sigma v t s l mgu:
-  acyclic s -> v \notin domf s -> v \notin vars t -> domf s # vars t ->
+  idempotent s -> v \notin domf s -> v \notin vars t -> domf s # vars t ->
   mgu_help (deref_sigma v t s) mgu (deref_list v t l) ->
   mgu_help s mgu ((Tm_V v, t) :: l).
 Proof.
@@ -235,7 +235,7 @@ Proof.
       case: fndP => //v2m; [rewrite in_fnd|rewrite not_fnd//].
       by rewrite ffunE valPE/= derefkv_not_in//.
     exists (deref_sigma v' (Tm_V v) r).
-      apply: acyclic_sigma_deref_sigma => //; first by rewrite inE eq_sym.
+      apply: idempotent_deref_sigma => //; first by rewrite inE eq_sym.
       by rewrite /=fdisjointX1.
     elim => //[v2|/=?->?->//].
     rewrite !deref_V fnd_set; case: eqP => vv2; subst.
@@ -280,7 +280,7 @@ Proof.
 Qed.
 
 
-Lemma montanariPmgu b l s mgu: acyclic s -> disjoint_L s l ->
+Lemma montanariPmgu b l s mgu: idempotent s -> disjoint_L s l ->
   montanari s b l = Some mgu -> mgu_help s mgu l.
 Proof.
   move: mgu; montanari_ind s b l => mgu A//; cycle -1.
@@ -294,24 +294,24 @@ Proof.
     apply/mgu_help_app/IH; auto.
     by rewrite !disjoint_L_cons/=d1 d2 d3 d4.
   - rewrite disjoint_L_cons/= => /and3P[D1 D2 D3] M.
-    have {M IH} := IH _ (acyclic_sigma_deref_sigma _ _ A) (disjoint_deref_sigma_deref_list A _ _ _) M.
+    have {M IH} := IH _ (idempotent_deref_sigma _ _ A) (disjoint_deref_sigma_deref_list A _ _ _) M.
     rewrite inE in vt.
     rewrite inE/= eq_sym => /(_ vt D1 D1 vt D3) IH.
     apply: mgu_help_cons_comm; rewrite !fdisjointX1 in D1, D2.
     by apply: mgu_help_deref_sigma IH; rewrite//(inE,fdisjointX1)//eq_sym.
   - rewrite disjoint_L_cons/= => /and3P[D1 D2 D3] M.
-    have {M}IH := IH _ (acyclic_sigma_deref_sigma vt D2 A) (disjoint_deref_sigma_deref_list A D2 vt D3) M.
+    have {M}IH := IH _ (idempotent_deref_sigma vt D2 A) (disjoint_deref_sigma_deref_list A D2 vt D3) M.
     by apply: mgu_help_deref_sigma IH; rewrite fdisjointX1 in D1. 
 Qed.
 
 Definition mgu m t1 t2 :=
-  acyclic m /\ deref m t1 = deref m t2 /\ forall s, acyclic s -> deref s t1 = deref s t2 -> 
-    exists s', acyclic s' /\ forall t, deref s' (deref m t) = (deref s t).
+  idempotent m /\ deref m t1 = deref m t2 /\ forall s, idempotent s -> deref s t1 = deref s t2 -> 
+    exists s', idempotent s' /\ forall t, deref s' (deref m t) = (deref s t).
 
 Lemma ren_empty t: ren fmap0 t = t.
 Proof. elim: t => //=[v|f -> a ->]//; rewrite not_fnd//. Qed.
 
-Lemma is_mgu0 s: acyclic s -> is_mgu fmap0 s.
+Lemma is_mgu0 s: idempotent s -> is_mgu fmap0 s.
 Proof. by exists s => //t; rewrite deref_empty. Qed.
 
 (*SNIPT: unif_correct *)
@@ -320,10 +320,10 @@ Lemma unify_correct t1 t2 s:
 (*ENDSNIPT: unif_correct *)
 Proof.
   move=> U.
-  have H := montanariPmgu acyclic_sigma0 (disjoint_Lempty _) U.
+  have H := montanariPmgu idempotent_0 (disjoint_Lempty _) U.
   rewrite !deref_empty in H; repeat split.
-    by apply: unif_acyclic acyclic_sigma0 U.
-    by have:= unify_P acyclic_sigma0 U.
+    by apply: unif_idempotent idempotent_0 U.
+    by have:= unify_P idempotent_0 U.
   move=> s' A D.
   have:= H s' A; rewrite/=/unif_pair/map_prod1 D eqxx.
   move=> /(_ isT (is_mgu0 _)) [|r] //.
@@ -334,12 +334,12 @@ Print Assumptions mgu_help_deref_sigma.
 
 (*SNIPT: unify_complete *)
 Lemma unify_complete:
-  forall t1 t2, (exists s, acyclic s /\ deref s t1 = deref s t2) -> exists s', unify t1 t2 fmap0 = Some s'.
+  forall t1 t2, (exists s, idempotent s /\ deref s t1 = deref s t2) -> exists s', unify t1 t2 fmap0 = Some s'.
 (*ENDSNIPT: unify_complete *)
 Proof.
   move=> t1 t2 [sx [H1 H2]].
   rewrite /unify/montanari_deref/montanari_pair.
-  have:= exists_montanari acyclic_sigma0 (disjoint_Lempty _) (ex_intro _ sx _).
+  have:= exists_montanari idempotent_0 (disjoint_Lempty _) (ex_intro _ sx _).
   move=> /(_ fset0 [::(deref fmap0 t1, deref fmap0 t2)] ).
   rewrite H1/= /unif_pair/map_prod1/= !deref_empty H2 eqxx fdisjointX0.
   move=> /(_ (And3 isT isT isT)).
